@base <http://w3id.org/openeduhub/vocabs/accessibilitySummary/> .
@prefix dct: <http://purl.org/dc/terms/> .
@prefix skos: <http://www.w3.org/2004/02/skos/core#> .
@prefix xsd: <http://www.w3.org/2001/XMLSchema#> .

<> a skos:ConceptScheme ;
    dct:title "Barrierefreiheit"@de ;
    dct:title "Accessibility"@en ;
    dct:description "Accessibility rating of some content. If a concept X is narrower than a concept Y, then that means that the rating X has higher requirements. I.e. the follow a partial ordering."@en ;
    dct:creator "<https://wirlernenonline.de>" ;
    dct:created "2020-11-16"^^xsd:date ;
    dct:modified "2022-07-19"^^xsd:date ;
    dct:issued "2020-11-16"^^xsd:date ;
    dct:license <http://creativecommons.org/publicdomain/zero/1.0/> ;
    skos:hasTopConcept <b>, <a>, <aa>, <aaa>, <bitv-I>, <bitv-II> .

<b> a skos:Concept ;
    skos:prefLabel "B" ;
    skos:definition "The content does not comply to the WCAG A rating requirements."@en ;
    skos:definition "Der Inhalt erfüllt nicht die WCAG Anforderungen für eine A-Wertung."@en ;
    skos:topConceptOf <> .

<a> a skos:Concept ;
    skos:prefLabel "WCAG-A";
    skos:definition "The content does comply to the WCAG A rating requirements."@en ;
    skos:definition "Der Inhalt erfüllt die WCAG Anforderungen für eine A-Wertung."@en ;
    skos:narrower <b> ;
    skos:topConceptOf <> .

<aa> a skos:Concept ;
    skos:prefLabel "WCAG-AA" ;
    skos:definition "The content does comply to the WCAG AA rating requirements."@en ;
    skos:definition "Der Inhalt erfüllt die WCAG Anforderungen für eine AA-Wertung."@en ;
    skos:narrower <aa> ;
    skos:topConceptOf <> .

<aaa> a skos:Concept ;
    skos:prefLabel "WCAG-AAA" ;
    skos:definition "The content does comply to the WCAG AAA rating requirements."@en ;
    skos:definition "Der Inhalt erfüllt die WCAG Anforderungen für eine AAA-Wertung."@en ;
    skos:narrower <aaa> ;
    skos:topConceptOf <> .

<bitv-I> a skos:Concept ;
    skos:prefLabel "BITV I";
    skos:definition "The content does comply to the BITV 2.0 Priority I requirements."@en ;
    skos:definition "Der Inhalt erfüllt die BITV 2.0 Priorität I Anforderungen für eine AAA-Wertung."@en ;
    skos:narrower <aa> ;
    skos:topConceptOf <> .

<bitv-II> a skos:Concept ;
    skos:prefLabel "BITV II";
    skos:definition "The content does comply to the BITV 2.0 Priority II requirements."@en ;
    skos:definition "Der Inhalt erfüllt die BITV 2.0 Priorität II Anforderungen für eine AAA-Wertung."@en ;
    skos:narrower <aaa> ;
    skos:narrower <bitv-I> ;
    skos:topConceptOf <> .