@prefix audRole: <http://purl.org/dcx/lrmi-vocabs/educationalAudienceRole/> .
@prefix dc: <http://purl.org/dc/elements/1.1/> .
@prefix dct: <http://purl.org/dc/terms/> .
@prefix rdf: <http://www.w3.org/1999/02/22-rdf-syntax-ns#> .
@prefix rdfs: <http://www.w3.org/2000/01/rdf-schema#> .
@prefix skos: <http://www.w3.org/2004/02/skos/core#> .
@prefix skosxl: <http://www.w3.org/2008/05/skos-xl#> .
@prefix xml: <http://www.w3.org/XML/1998/namespace> .
@prefix xsd: <http://www.w3.org/2001/XMLSchema#> .

audRole: a skos:ConceptScheme;
  dc:title "LRMI Educational Audience Role Vocabulary" ;
  dc:creator "LRMI Task Group (DCMI)"@en;
  dct:description "A concept scheme that defines the primary or intended roles of the audience (beneficiary) of the resource being described."@en;
  dct:created "2017-03-01"^^xsd:date ;
  dct:modified "2020-04-08"^^xsd:date ;  
  dct:license <http://creativecommons.org/licenses/by/4.0/> .  
  
audRole:administrator a skos:Concept;
  skos:prefLabel "administrator"@en;
  skos:prefLabel "administrator"@de;
  skos:altLabel "admin"@en;
  skos:altLabel "admin"@de;
  skos:altLabel "admins"@de;
  skos:definition "A trainer or educator with administrative authority and responsibility."@en-US;
  skos:definition "Ein Trainer oder Pädagoge mit administrativer Autorität und Verantwortung."@de;
  skos:inScheme audRole: .

audRole:generalPublic a skos:Concept;
  skos:prefLabel "general public"@en;
  skos:prefLabel "allgemeine Öffentlichkeit"@de;
  skos:altLabel "Öffentlichkeit"@de;
  skos:definition "The public at large."@en;
  skos:inScheme audRole: .
  
audRole:mentor a skos:Concept;
  skos:prefLabel "mentor"@en;  
  skos:prefLabel "Mentor"@de;
  skos:altLabel "Ratgeber"@de;
  skos:definition "Someone who advises, trains, supports, and/or guides."@en;
  skos:inScheme audRole: .  

audRole:parent a skos:Concept;
  skos:prefLabel "parent"@en;
  skos:prefLabel "Eltern"@de;
  skos:altLabel "Elter"@de;
  skos:altLabel "Elternteil"@de;
  skos:altLabel "Erziehungsberechtigter"@de;
  skos:altLabel "Sorgeberechtigter"@de;
  skos:definition "A father, mother, or legal guardian."@en;
  skos:inScheme audRole: .
  
audRole:peerTutor a skos:Concept;
  skos:prefLabel "peer tutor"@en;
  skos:prefLabel "Nachhilfe"@de;
  skos:altLabel "Nachhilfelehrerin"@de;
  skos:altLabel "Nachhilfelehrer"@de;
  skos:definition "The peer learner serving as tutor of another learner."@en;
  skos:broader audRole:student;
  skos:inScheme audRole: .

audRole:professional a skos:Concept;
  skos:prefLabel "professional"@en;
  skos:prefLabel "Profi"@de;
  skos:altLabel "Fachfrau"@de;
  skos:altLabel "Fachmann"@de;
  skos:definition "Someone already practicing a profession; an industry partner, or professional development trainer."@en;
  skos:inScheme audRole: .
       
audRole:student a skos:Concept;
  skos:prefLabel "student"@en;
  skos:prefLabel "Schüler"@de;
  skos:altLabel "Schülerin"@de;
  skos:altLabel "Lernende"@de;
  skos:altLabel "Lernender"@de;
  skos:altLabel "students"@en;
  skos:definition "The learner or trainee."@en;
  skos:narrower audRole:peerTutor;
  skos:inScheme audRole: .
       
audRole:teacher a skos:Concept;
  skos:prefLabel "teacher"@en;
  skos:prefLabel "Lehrer"@de;
  skos:altLabel "Lehrerin"@de;
  skos:altLabel "Lehrende"@de;
  skos:altLabel "Lehrender"@de;
  skos:definition "A person who has been trained to implement educational methods and practices."@en ;
  skos:inScheme audRole: .            